Reworked basic definitions.
* Removed Variable fake string, replaced with tagged type families.

* Made Felt inhabited with arbitrary -42 - adjusted Op.run accordingly
  to use get!, which significantly reduces definition clutter and
  casing.

* Restated definitions in terms of notations, renamed for consistency.

* Restructured lemmas altogether - we now have a minimal set of lemmas
  necessary. Note further all '_Op_Seq_Collapsibles' are *gone*.
  They are now simply composition of '_Op' and '_Seq'.

* Rewrote the MLIR tactic to use the new set of simplified lemmas,
  massaged proofs to go through.

Is0/Basic.lean
@@ -27,7 +27,7 @@ namespace Map
 
 section Map
 
-variable {α : Type} [BEq α] [DecidableEq α] {β : Type}
+variable {α : Type} [DecidableEq α] {β : Type}
 
 def empty : Map α β := λ _ => none
 
@@ -39,7 +39,7 @@ def fromList (l : List (α × β)) : Map α β :=
   | [] => Map.empty
   | (k, v) :: xs => Map.update (Map.fromList xs) k v
 
-notation:61 st "[" n:61 "]" " := " x:49 => Map.update st n x
+notation:61 m "[" k:61 "]" " := " v:49 => Map.update m k v
 
 @[simp]
 lemma fromList_nil : fromList ([] : List (α × β)) = Map.empty := rfl
@@ -89,18 +89,19 @@ lemma State.update_constraint {state : State} {name : String} {c : Prop} :
 
 @[simp]
 lemma State.if_constraints {state₁ state₂ : State} {x : Felt} :
-  (if (x = 0) then state₁ else state₂).constraints = if (x = 0) then state₁.constraints else state₂.constraints := by
-  exact apply_ite constraints (x = 0) state₁ state₂
+  (if x = 0 then state₁ else state₂).constraints =
+  if x = 0 then state₁.constraints else state₂.constraints := by apply apply_ite
 
 @[simp]
 lemma State.if_output {state₁ state₂ : State} {x : Felt} :
-  (if (x = 0) then state₁ else state₂).output = if (x = 0) then state₁.output else state₂.output := by
-  exact apply_ite output (x = 0) state₁ state₂
+  (if x = 0 then state₁ else state₂).output =
+  if (x = 0) then state₁.output else state₂.output := by apply apply_ite
 
 notation:61 st "[" n:61 "]" " := " x:49 => State.update st n x
 
--- A parametrized Variable. In practice, α will be one of `Felt`, `Prop`, or `List Felt`.
-structure Variable (α : Type) :=
+inductive VarType := | FeltTag | PropTag | ListFeltTag
+
+structure Variable (tag : VarType) :=
   name : String
 
 inductive IsNondet :=
@@ -116,22 +117,23 @@ def lub (x₁ x₂ : IsNondet) :=
     | _ => x₂
 
 -- Pure functional operations from the cirgen (circuit generation) MLIR dialect.
+open VarType in
 inductive Op : IsNondet → Type where
   | Const : Felt → Op x
   | True : Op x
   | GetInput : ℕ → Felt → Op x
   | GetOutput : ℕ → Felt → Op x
-  | Sub : Variable Felt → Variable Felt → Op x
-  | Mul : Variable Felt → Variable Felt → Op x
-  | AndEqz : Variable Prop → Variable Felt → Op x
-  | AndCond : Variable Prop → Variable Felt → Variable Prop → Op x
-  | Isz : Variable Felt → Op InNondet
-  | Inv : Variable Felt → Op InNondet
+  | Sub : Variable FeltTag → Variable FeltTag → Op x
+  | Mul : Variable FeltTag → Variable FeltTag → Op x
+  | AndEqz : Variable PropTag → Variable FeltTag → Op x
+  | AndCond : Variable PropTag → Variable FeltTag → Variable PropTag → Op x
+  | Isz : Variable FeltTag → Op InNondet
+  | Inv : Variable FeltTag → Op InNondet
 
-open Op
+open Op VarType
 
-instance {x : IsNondet} : HSub (Variable Felt) (Variable Felt) (Op x) := ⟨Op.Sub⟩
-instance {x : IsNondet} : HMul (Variable Felt) (Variable Felt) (Op x) := ⟨Op.Mul⟩
+instance {x : IsNondet} : HSub (Variable FeltTag) (Variable FeltTag) (Op x) := ⟨Op.Sub⟩
+instance {x : IsNondet} : HMul (Variable FeltTag) (Variable FeltTag) (Op x) := ⟨Op.Mul⟩
 
 -- Notation for Ops.
 namespace MLIRNotation
@@ -147,48 +149,33 @@ scoped prefix:max "Inv" => Op.Inv
 
 end MLIRNotation
 
+instance : Inhabited Felt := ⟨-42⟩
+
 -- Evaluate a pure functional circuit operation to get some kind of literal.
-def Op.eval {x} (state : State) (op : Op x) : Lit :=
+def Op.eval {x} (st : State) (op : Op x) : Lit :=
   match op with
-  | Const x => .Val x
-  | True => .Constraint (_root_.True)
-  | GetInput i _ => .Val <| state.input.getD i (-42)
-  | GetOutput i _ => .Val <| state.output.getD i (-42)
-  | Sub x y => .Val $ match state.felts x.name, state.felts y.name with
-                        | some x, some y => x - y
-                        | _      , _       => 42
-  | Mul x y => .Val $ match state.felts x.name, state.felts y.name with
-                        | some x, some y => x * y
-                        | _      , _       => 42
-  | AndEqz c x => .Constraint $ match state.props c.name, state.felts x.name with
-                    | some c, some x => c ∧ x = 0
-                    | _      , _     => 42 = 42
+  | Const x       => .Val x
+  | True          => .Constraint _root_.True
+  | GetInput i _  => .Val <| st.input.get! i
+  | GetOutput i _ => .Val <| st.output.get! i
+  | Sub x y       => .Val <| (st.felts x.name).get! - (st.felts y.name).get!
+  | Mul x y       => .Val <| (st.felts x.name).get! * (st.felts y.name).get!
+  | AndEqz c x    => .Constraint <| (st.props c.name).get! ∧ (st.felts x.name).get! = 0
   | AndCond old cond inner =>
-      .Constraint $ match state.props old.name, state.felts cond.name, state.props inner.name with
-        | .some old, .some cond, .some inner => if cond == 0 then old else old ∧ inner
-        | _        , _         , _           => 42 = 42
-  | Isz x => .Val $ match state.felts x.name with
-               | some x => if x == 0 then 1 else 0
-               | _      => 42
-  | Inv x => .Val $ match state.felts x.name with
-               | some x => if x == 0 then 0 else x⁻¹
-               | _      => 42
+      .Constraint <| (st.props old.name).get! ∧
+                     if (st.felts cond.name).get! = 0
+                       then _root_.True
+                       else (st.props inner.name).get!
+  | Isz x         => .Val $ if (st.felts x.name).get! = 0 then 1 else 0
+  | Inv x         => .Val $ match st.felts x.name with
+                              | some x => if x = 0 then 0 else x⁻¹
+                              | _      => default
 
 notation:61 "Γ " st:max " ⟦" p:49 "⟧ₑ" => Op.eval st p
 
--- open MLIR in
--- lemma x : MLIRProgram := Sequence (Nondet (Assign "x" (Op.Isz ⟨"y"⟩))) (Assign "z" (Op.Const 4))
-
--- open MLIR in
--- lemma y : MLIR InNondet := Sequence ((Assign "x" (Op.Isz ⟨"y"⟩))) ((Assign "z" (Op.Const 4)))
-
 namespace MLIRNotation
 
--- scoped notation:56 (priority := high) "[" x "]" => ⟨x⟩
-
 end MLIRNotation
-
--- instance : Inhabited Lit := ⟨(Lit.Val (-42))⟩
 
 namespace Op
 
@@ -196,62 +183,45 @@ section Op
 
 open MLIRNotation
 
-variable (st : State) {α : IsNondet}
+variable {st : State} {α : IsNondet}
 
 @[simp]
-lemma eval_const {x : Felt} : Γ st ⟦@Const α x⟧ₑ = .Val x := rfl
+lemma eval_const : Γ st ⟦@Const α x⟧ₑ = .Val x := rfl
 
 @[simp]
 lemma eval_true : Γ st ⟦@Op.True α⟧ₑ = .Constraint (_root_.True) := rfl
 
 @[simp]
-lemma eval_getInput {i : ℕ} {x : Felt} : Γ st ⟦@GetInput α i x⟧ₑ = .Val (st.input.getD i (-42)) := rfl
+lemma eval_getInput : Γ st ⟦@GetInput α i x⟧ₑ = .Val (st.input.get! i) := rfl
 
 @[simp]
-lemma eval_getOutput {i : ℕ} {x : Felt} : Γ st ⟦@GetOutput α i x⟧ₑ = .Val (st.output.getD i (-42)) := rfl
+lemma eval_getOutput : Γ st ⟦@GetOutput α i x⟧ₑ = .Val (st.output.get! i) := rfl
 
 @[simp]
-lemma eval_sub {x y : Variable Felt} :
-  Γ st ⟦@Sub α x y⟧ₑ = .Val (match st.felts x.name, st.felts y.name with
-                              | some x, some y => x - y
-                              | _      , _     => 42) := rfl
+lemma eval_sub : Γ st ⟦@Sub α x y⟧ₑ = .Val ((st.felts x.name).get! - (st.felts y.name).get!) := rfl
 
 @[simp]
-lemma eval_mul {x y : Variable Felt} :
-  Γ st ⟦@Mul α x y⟧ₑ = .Val (match st.felts x.name, st.felts y.name with
-                              | some x, some y => x * y
-                              | _      , _     => 42) := rfl
+lemma eval_mul : Γ st ⟦@Mul α x y⟧ₑ = .Val ((st.felts x.name).get! * (st.felts y.name).get!) := rfl
 
 @[simp]
-lemma eval_isz {x : Variable Felt} :
-  Γ st ⟦??₀x⟧ₑ = .Val (match st.felts x.name with
-                        | some x => if x == 0 then 1 else 0
-                        | _      => 42) := rfl
-@[simp]
-lemma eval_inv {x : Variable Felt} :
-  Γ st ⟦Inv x⟧ₑ = .Val (match st.felts x.name with
-                         | some x => if x == 0 then 0 else x⁻¹
-                         | _      => 42) := rfl
-
--- lemma eval_eqz {c : Variable Prop}
---                {x : Variable Felt}
---     (h₁ : state.props c.name = some c₁)
---     (h₂ : state.felts x.name = some x₁) :
---   (AndEqz c x).eval state = .Constraint (c₁ ∧ x₁ = 0) := by simp [eval, *]
+lemma eval_isz : Γ st ⟦??₀x⟧ₑ = .Val (if (st.felts x.name).get! = 0 then 1 else 0) := rfl
 
 @[simp]
-lemma eval_andEqz :
-  Γ st ⟦@AndEqz α c x⟧ₑ =
-    .Constraint (match st.props c.name, st.felts x.name with
-                   | some c, some x => (c ∧ x = 0)
-                   | _      , _     => (42 = 42)) := rfl
+lemma eval_inv : Γ st ⟦Inv x⟧ₑ = .Val (match st.felts x.name with
+                                        | some x => if x = 0 then 0 else x⁻¹
+                                        | _      => default) := rfl
+
+@[simp]
+lemma eval_andEqz : Γ st ⟦@AndEqz α c x⟧ₑ =
+                    .Constraint ((st.props c.name).get! ∧ (st.felts x.name).get! = 0) := rfl
 
 @[simp]
 lemma eval_andCond :
   Γ st ⟦@AndCond α old cnd inner⟧ₑ =
-    .Constraint (match st.props old.name, st.felts cnd.name, st.props inner.name with
-                  | .some old, .some cnd, .some inner => if cnd == 0 then old else old ∧ inner
-                  | _        , _         , _           => 42 = 42) := rfl
+    .Constraint ((st.props old.name).get! ∧
+                 if (st.felts cnd.name).get! = 0
+                   then _root_.True
+                   else (st.props inner.name).get!) := rfl
 
 end Op
 
@@ -259,11 +229,11 @@ end Op
 
 inductive MLIR : IsNondet → Type where
   | Assign : String → Op x → MLIR x
-  | Eqz : Variable Felt → MLIR x
-  | If : Variable Felt → MLIR x → MLIR x
+  | Eqz : Variable FeltTag → MLIR x
+  | If : Variable FeltTag → MLIR x → MLIR x
   | Nondet : MLIR InNondet → MLIR NotInNondet
   | Sequence : MLIR x → MLIR x → MLIR x
-  | SetOutput : ℕ → Variable Felt → MLIR InNondet
+  | SetOutput : ℕ → Variable FeltTag → MLIR InNondet
 
 -- Notation for MLIR programs.  
 namespace MLIRNotation
@@ -279,62 +249,36 @@ end MLIRNotation
 
 abbrev MLIRProgram := MLIR NotInNondet
 
--- Evaluate `op` and map `name ↦ result` in `state : State`.
-def Op.assign {α} (state : State) (op : Op α) (name : String) : State :=
-  match (Op.eval state op) with
-  | .Val x => { state with felts := state.felts.update name x }
-  | .Constraint c => { state with props := state.props.update name c }
+abbrev withEqZero (x : Felt) (st : State) : State :=
+  {st with constraints := (x = 0) :: st.constraints}
 
--- inductive MLIR : IsNondet → Type where
---   | Assign : String → Op x → MLIR x
---   | Eqz : Variable Felt → MLIR x
---   | If : Variable Felt → MLIR x → MLIR x
---   | Nondet : MLIR InNondet → MLIR NotInNondet
---   | Sequence : MLIR x → MLIR x → MLIR x
---   | SetOutput : Variable Felt → Op x → MLIR InNondet
+@[simp]
+lemma withEqZero_def : withEqZero x st = {st with constraints := (x = 0) :: st.constraints} := rfl
 
 -- Step through the entirety of a `MLIR` MLIR program from initial state
 -- `state`, yielding the post-execution state and possibly a constraint
 -- (`Prop`), the return value of the program.
-def MLIR.run {α} (program : MLIR α) (st : State) : State :=
+def MLIR.run {α : IsNondet} (program : MLIR α) (st : State) : State :=
   match program with
-  | Assign name op => Op.assign st op name
-  | Eqz x =>
-    match st.felts x.name with
-      | .some x => {st with constraints := (x = 0) :: st.constraints}
-      | .none   => st
-  | If x program =>
-    match st.felts x.name with
-      | some x => if x == 0
-                  then st
-                  else MLIR.run program st
-      | none    => st
-  | Nondet block => MLIR.run block st
-  | Sequence a b => let st' := MLIR.run a st
-                    MLIR.run b st'
-  | SetOutput i x =>
-    match st.felts x.name with
-      | .some x => {st with output := st.output.set i x}
-      | _       => st
+    | Assign name op => st[name] := Γ st ⟦op⟧ₑ
+    | Eqz x =>
+        match st.felts x.name with
+          | .some x => withEqZero x st
+          | _       => st
+    | If x program =>
+        match st.felts x.name with
+          | some x => if x = 0 then st else program.run st
+          | _      => st
+    | Nondet block => block.run st
+    | Sequence a b => b.run (a.run st)
+    | SetOutput i x =>
+        match st.felts x.name with
+          | .some x => {st with output := st.output.set i x}
+          | _       => st
 
-@[simp, reducible]
-abbrev MLIR.runProgram (program : MLIRProgram) := MLIR.run program
+@[simp]
+abbrev MLIR.runProgram (program : MLIRProgram) := program.run
 
 notation:61 "Γ " st:max " ⟦" p:49 "⟧" => MLIR.run p st
-
--- lemma run_setOutput_of_some
---   {state : State}
---   {i : ℕ}
---   {x₁ : Felt}
---   {x : Variable Felt}
---   (h : state.felts x.name = some x₁) :
---   Γ state ⟦MLIR.SetOutput i x⟧ = {state with output := state.output.set i x₁} := by simp [MLIR.run, h]
-
--- lemma run_Eqz_of_some
---   {state : State}
---   {x₁ : Felt}
---   {x : Variable Felt}
---   (h : state.felts x.name = some x₁) :
---   Γ state ⟦MLIR.Eqz x⟧ = {state with constraints := (x₁ = 0) :: state.constraints } := by simp [MLIR.run, h]
 
 end Risc0
