Is0.lean
@@ -2,3 +2,4 @@ import Is0.Basic
 import Is0.Is0
 import Is0.Lemmas
 import Is0.Programs
+import Is0.Wheels
