Is0/Lemmas.lean
@@ -12,103 +12,30 @@ section WithMLIR
 
 variable {α : IsNondet} {st : State} {name : String}
 
-open MLIRNotation
-open IsNondet
+open MLIRNotation IsNondet
+open Risc0.VarType
 
-lemma MLIR.run_assign :
-  Γ st ⟦name ←ₐ op⟧ = st[name] := op.eval st := rfl
+-- MLIR.run def lemmas
+lemma MLIR.run_ass_def : Γ st ⟦name ←ₐ op⟧ = st[name] := Γ st ⟦op⟧ₑ := rfl
 
-lemma MLIR.run_Sequence_Assign_collapsible {op : Op α} {program : MLIR α} :
-    Γ st ⟦name ←ₐ op; program⟧ = Γ (st[name] := Op.eval st op) ⟦program⟧ := by
-  cases op <;> conv => lhs; simp [MLIR.run, State.update, Map.update, beq_iff_eq]
-
-lemma MLIR.run_set : Γ st ⟦MLIR.SetOutput i x⟧ = 
+lemma MLIR.run_set_def : Γ st ⟦output[i] ←ᵢ x⟧ = 
   match st.felts x.name with
     | .some x => {st with output := st.output.set i x}
     | _       => st := rfl
 
-lemma MLIR.run_Sequence_Set_collapsible
-    {nameₓ : String}
-    {program : MLIR InNondet}
-    (x : Felt)
-    (h₁ : st.felts nameₓ = some x) :
-    Γ st ⟦output[i] ←ᵢ ⟨nameₓ⟩; program⟧ = 
-    Γ { st with output := st.output.set i x } ⟦program⟧ := by simp [run, *]
+lemma MLIR.run_seq_def : Γ st ⟦p₁; p₂⟧ = Γ (Γ st ⟦p₁⟧) ⟦p₂⟧ := rfl
 
-lemma MLIR.run_Set_collapsible
-    {nameₓ : String}
-    (x : Felt)
-    (h₁ : st.felts nameₓ = some x) :
-    Γ st ⟦output[i] ←ᵢ ⟨nameₓ⟩⟧ = 
-    { st with output := st.output.set i x } := by simp [run, *]
+lemma MLIR.run_nondet : Γ st ⟦nondet block⟧ = Γ st ⟦block⟧ := rfl
 
-lemma MLIR.run_if_true {c : Variable Felt}
-  (h : st.felts c.name = some 0) :
-  Γ st ⟦guard c then prog⟧ = st := by
-  simp only [run]; generalize eq : st.felts c.name = cond
-  rcases cond with _ | ⟨x⟩ <;> simp only
-  rw [eq] at h
-  cases h
-  simp only
-  simp only [ite_true]
+lemma MLIR.run_set (x : Felt) (h₁ : st.felts nameₓ = some x) :
+  Γ st ⟦output[i] ←ᵢ ⟨nameₓ⟩⟧ = { st with output := st.output.set i x } := by simp [run_set_def, h₁]
 
-lemma MLIR.run_if_false {c : Variable Felt}
-  (x : Felt)
-  (h₁ : st.felts c.name = some x)
-  (h₂ : x ≠ 0) :
-  Γ st ⟦guard c then prog⟧ = Γ st ⟦prog⟧ := by
-  simp only [run]; generalize eq : st.felts c.name = cond
-  rcases cond with _ | ⟨y⟩ <;> simp only <;> rw [eq] at h₁
-  · cases h₁
-  · simp; intros contra
-    rw [contra] at h₁
-    injection h₁ with contra
-    exact absurd contra.symm h₂
+lemma MLIR.run_if (x : Felt) (h₁ : st.felts name = some x) :
+  Γ st ⟦guard ⟨name⟩ then branch⟧
+  = if x = 0 then st else Γ st ⟦branch⟧ := by simp [run, h₁]
 
-lemma MLIR.run_seq :
-  Γ st ⟦p₁; p₂⟧ = Γ (Γ st ⟦p₁⟧) ⟦p₂⟧ := rfl
-
-lemma MLIR.run_Sequence_If_collapsible
-    {branch : MLIR α}
-    {program : MLIR α}
-    (x : Felt)
-    (h₁ : st.felts name = some x)
-    : Γ st ⟦guard ⟨name⟩ then branch; program⟧
-  = if (x == 0)
-      then Γ st ⟦program⟧
-      else Γ st ⟦branch; program⟧ := by
-    generalize eq : (x == 0) = cond
-    rw [run_seq]
-    rcases cond with _ | _ <;> simp only
-    · rw [run_if_false x h₁ (by simp at eq; exact eq)]; rfl
-    · rw [run_if_true (by simp at eq; rw [eq] at h₁; exact h₁)]; rfl
-
-lemma MLIR.run_If_collapsible
-    {branch : MLIR α}
-    (x : Felt)
-    (h₁ : st.felts name = some x) :
-    Γ st ⟦guard ⟨name⟩ then branch⟧
-  = if (x == 0)
-      then st
-      else Γ st ⟦branch⟧ := by simp [run, h₁]
-
-lemma MLIR.run_Sequence_nondet_collapsible :
-  Γ st ⟦nondet block; program⟧ = Γ (Γ st ⟦block⟧) ⟦program⟧ := rfl
-
-lemma MLIR.run_Eqz_collapsible
-    (x : Felt)
-    (h₁ : st.felts name = some x) :
-    Γ st ⟦@MLIR.Eqz α ⟨name⟩⟧ 
-  = { st with constraints := (x = 0) :: st.constraints } := by simp [run, *]
-
-lemma MLIR.run_Sequence_Eqz_collapsible
-    {program : MLIR α}
-    (x : Felt)
-    (h₁ : st.felts name = some x) :
-    Γ st ⟦.Sequence (.Eqz (Variable.mk name)) program⟧
-  = let state₁ := { st with constraints := (x = 0) :: st.constraints }
-    let state₂ := Γ state₁ ⟦program⟧
-    state₂ := by rw [run_seq, run_Eqz_collapsible _ h₁]
+lemma MLIR.run_eqz (x : Felt) (h₁ : st.felts name = some x) :
+  Γ st ⟦@MLIR.Eqz α ⟨name⟩⟧ = withEqZero x st := by simp [run, h₁]
 
 end WithMLIR 
 
