Is0/Wheels.lean
@@ -1,0 +1,15 @@
+namespace Risc0
+
+namespace Wheels
+
+namespace Option
+
+@[simp]
+theorem get_some {α : Type} [Inhabited α] {x : α} :
+  @Option.get! α _ (some x) = x := rfl
+
+end Option
+
+end Wheels
+
+end Risc0
